Fix DVE proof

DVE.v
@@ -67,6 +67,8 @@ Proof.
   rewrite zip_map_fst; eauto with len.
 Qed.
 
+Require Import paco2.
+
 (* A proof relation is parameterized by analysis information A *)
 Class ProofRelationI (A:Type) := {
     (* Relates parameter lists according to analysis information *)
@@ -223,150 +225,6 @@ Proof.
   eapply renILabenv_extension'; eauto using renILabenv_mon, indexwise_r_mon.
 Qed.
 
-(*
-Definition indexwise_r' (r:rel2 I.state (fun _ => I.state)) A (PR:ProofRelationI A) AL L L' :=
-  forall f f' a Z s n Z' s' n',
-    IndexRelI AL f f'
-    -> get AL f a
-    -> get L f (I.blockI Z s n)
-    -> get L' f' (I.blockI Z' s' n')
-    -> forall E E' VL VL',
-        ArgRelI E E' a VL VL'
-        -> r (drop (f - n) L, E[Z <-- List.map Some VL], s)
-            (drop (f' - n') L', E'[Z' <-- List.map Some VL'], s').
-
-Lemma indexwise_r_mon' (r r':rel2 I.state (fun _ => I.state)) A (PR:ProofRelationI A) AL' F F' AL L L'
-  : indexwise_r r PR AL' F F' AL L L'
-    -> (forall x y, r x y -> r' x y)
-    -> indexwise_r r' PR AL' F F' AL L L'.
-Proof.
-  intros Idx LE; hnf; intros; eauto.
-Qed.
-
-Definition indexwise_proofrel' A (PR:ProofRelationI A) AL L L' :=
-  forall f f' Z s n Z' s' n' a,
-    IndexRelI AL f f'
-    -> get L f (I.blockI Z s n)
-    -> get L' f' (I.blockI Z' s' n')
-    -> get AL f a
-    -> ParamRelI a Z Z' /\ BlockRelI a (I.blockI Z s n) (I.blockI Z' s' n').
-
-Lemma fix_compatible_I' A (PR:ProofRelationI A) AL L L'
-(LEN2:length AL = length L)
-  : (forall r, renILabenv r PR AL L L' -> indexwise_r' (sim'r r) PR AL L L')
-    -> indexwise_proofrel' PR AL L L'
-    -> sawtooth L
-    -> sawtooth L'
-    -> forall r, indexwise_r' (sim'r r) PR AL L L'.
-Proof.
-  intros ISIM IP STL STL' r; pcofix CIH.
-  eapply ISIM; eauto.
-  split; eauto.
-  intros. split; eauto.
-  intros. exploit IP; eauto; dcr.
-  exploit ArgLengthMatchI; eauto; dcr.
-  pone_step.
-  eapply (sawtooth_get STL H1). simpl. eapply omap_length in H4. congruence.
-  eapply (sawtooth_get STL' H2). simpl. eapply omap_length in H5. congruence.
-  simpl. right. orewrite (n - n = 0). orewrite (n' - n' = 0). simpl.
-  eapply CIH; eauto.
-Qed.
-
-Lemma fix_compatible_I'' A (PR:ProofRelationI A) AL F F' L L' AL'
-(LEN2:length AL' = length F)
-  : (forall r, renILabenv r PR (AL' ++ AL) (mapi I.mkBlock F ++ L) (mapi I.mkBlock F' ++ L')
-            -> indexwise_r (sim'r r) PR AL' F F' AL L L')
-    -> indexwise_proofrel PR F F' AL' AL
-    -> (forall n n', IndexRelI (AL' ++ AL) n n' -> n < length F -> n' < length F')
-    -> (forall n n', IndexRelI (AL' ++ AL) n n' -> n >= length F -> n' >= length F')
-    -> Image AL' = length F'
-    -> forall r, renILabenv r PR AL L L'
-           -> renILabenv (sim'r r) PR (AL' ++ AL) (mapi I.mkBlock F ++ L) (mapi I.mkBlock F' ++ L').
-Proof.
-  intros ISIM IP Ilt Ige Img r SIML.
-  destruct SIML as [[? ?] SIM].
-  exploit fix_compatible_I'; eauto using @sawtooth, tooth_I_mkBlocks with len.
-  intros.
-
-
-
-
-  eapply ISIM; eauto.
-  hnf. split.
-  destruct SIML; dcr; split; eauto with len. split.
-  econstructor; eauto. eapply tooth_I_mkBlocks.
-  econstructor; eauto. eapply tooth_I_mkBlocks.
-  eapply renILabenv_extension'; eauto using renILabenv_mon, indexwise_r_mon.
-Qed.
-
-
-Lemma renILabenv_extension' A (PR:ProofRelationI A) (AL:list A) L L'
-      (LEN1:length AL' = length F)
-  : (forall r, renILabenv r PR AL L L' -> indexwise_r' (sim'r r) PR AL L L')
-    -> indexwise_proofrel PR F F' AL' AL
-    -> (forall n n', IndexRelI (AL' ++ AL) n n' -> n < length F -> n' < length F')
-    -> (forall n n', IndexRelI (AL' ++ AL) n n' -> n >= length F -> n' >= length F')
-    -> Image AL' = length F'
-    -> forall r, renILabenv r PR AL L L'
-           -> renILabenv r PR (AL' ++ AL) (mapi I.mkBlock F ++ L) (mapi I.mkBlock F' ++ L').
-Proof.
-  intros. eapply renILabenv_extension'; eauto.
-  eapply indexwise_r_mon.
-  eapply fix_compatible_I; eauto. eauto.
-Qed.
-
-
-(*
-Lemma indexrel_extend A (PR:ProofRelationI A) AL F F' L L' AL'
-(LEN2:length AL' = length F)
-  : (forall n n', IndexRelI (AL' ++ AL) n n' -> n < length F -> n' < length F')
-    -> (forall n n', IndexRelI (AL' ++ AL) n n' -> n >= length F -> n' >= length F')
-    -> Image AL' = length F'
-    -> forall r, renILabenv r PR AL L L'
-           -> indexwise_r (sim'r r) PR AL' F F' AL L L'
-           -> indexwise_r' (sim'r r) PR (AL' ++ AL) (mapi I.mkBlock F ++ L) (mapi I.mkBlock F' ++ L').
-Proof.
-  intros Ilt Ige Img r SIML IW.
-  hnf. intros ? ? ? ? ? ? ? ? ? RN GetAL GetFL GetL'.
-  assert (❬AL'❭ = ❬mapi I.mkBlock F❭) by eauto with len.
-  eapply get_app_cases in GetAL. destruct GetAL as [GetAL'|GetAL].
-  - eapply get_app_lt_1 in GetFL; [| rewrite <- H; eauto using get_range].
-    inv_get. destruct x as [Z s]. simpl in *. clear EQ.
-    orewrite (n - n = 0). simpl.
-    exploit Ilt; eauto using get_range.
-    eapply get_app_lt_1 in GetL'; [| rewrite mapi_length; eauto with len ].
-    inv_get. destruct x as [Z' s']. simpl in *. clear EQ.
-    orewrite (n' - n' = 0); simpl.
-    eapply IW; eauto.
-  - destruct SIML; dcr.
-    exploit Ige; eauto; try congruence.
-    eapply get_app_right_ge in GetFL; [ | rewrite <- H; eauto].
-    eapply get_app_right_ge in GetL'; [ | eauto with len; rewrite mapi_length; eauto].
-    rewrite mapi_length in *.
-    eapply IndexRelDrop in RN; eauto.
-    edestruct H1 as [[? ?] SIM]; eauto. rewrite H; eauto. rewrite Img; eauto.
-    assert (f - n >= ❬mapi I.mkBlock F❭). {
-      exploit (sawtooth_smaller H7 GetFL).
-      rewrite <- H in *. rewrite mapi_length. simpl in *. omega.
-    }
-    assert (f' - n' >= ❬mapi I.mkBlock F'❭). {
-      exploit (sawtooth_smaller H6 GetL').
-      rewrite mapi_length in *.
-      simpl in *. omega.
-    }
-    rewrite (drop_app_gen _ (mapi I.mkBlock F)); eauto.
-    rewrite (drop_app_gen _ (mapi I.mkBlock F')); eauto.
-    repeat rewrite mapi_length. rewrite H in SIM. rewrite Img in SIM.
-    orewrite (f - n - ❬F❭ = f - ❬F❭ - n).
-    orewrite (f' - n' - ❬F'❭ = f' - ❬F'❭ - n').
-    eapply sim'_expansion_closed. eapply SIM; eauto.
-
-Admitted.
- *)
-
-*)
-
-
 Lemma renILabenv_extension A (PR:ProofRelationI A) (AL AL':list A) F F' L L'
       (LEN1:length AL' = length F)
   : (forall r, renILabenv r PR (AL' ++ AL) (mapi I.mkBlock F ++ L) (mapi I.mkBlock F' ++ L')
@@ -385,95 +243,87 @@ Qed.
 
 Module I.
 
-  Definition ArgRel (V V':onv val) (G:؟(set var) * params) (VL VL': list val) : Prop :=
-      VL' = (filter_by (fun x => B[x ∈ oget (fst G)]) (snd G) VL) /\
+  Definition ArgRel (V V':onv val) (G:(set var) * params) (VL VL': list val) : Prop :=
+      VL' = (filter_by (fun x => B[x ∈ fst G]) (snd G) VL) /\
       length (snd G) = length VL /\
-      agree_on eq (oget (fst G) \ of_list (snd G)) V V'.
+      agree_on eq (fst G \ of_list (snd G)) V V'.
 
 
-  Definition ParamRel (G:option (set var) * params) (Z Z' : list var) : Prop :=
-    Z' = (List.filter (fun x => B[x ∈ oget (fst G)]) Z) /\ snd G = Z.
+  Definition ParamRel (G:(set var) * params) (Z Z' : list var) : Prop :=
+    Z' = (List.filter (fun x => B[x ∈ fst G]) Z) /\ snd G = Z.
 
-Instance SR : ProofRelationI (؟(set var) * params) := {
+Instance SR : ProofRelationI ((set var) * params) := {
    ParamRelI := ParamRel;
    ArgRelI := ArgRel;
    BlockRelI := fun lvZ b b' => True;
-   Image AL := countSome (List.map fst AL);
-   IndexRelI AL n n' :=
-     n' = countSome (fst ⊝ (take n AL)) /\ exists lv Z, get AL n (Some lv, Z)
+   Image AL := length AL;
+   IndexRelI AL n n' := n = n'
 }.
 - intros. hnf in H, H0; dcr; subst.
   erewrite filter_filter_by_length; eauto.
-- intros AL' AL n n' [H H']; subst.
-  split. clear H' H.
-  + general induction AL'; simpl.
-    * orewrite (n - 0 = n). omega.
-    * destruct n; simpl; eauto. cases; simpl; eauto.
-  + destruct H' as [? [? ?]]. rewrite get_app_ge in H0; eauto.
+- intros AL' AL n n' H H'; subst; reflexivity.
 Defined.
 
 
-Lemma inv_extend s L L' LV als lv Z f
+Lemma inv_extend s L L' ZL LV als lv f
 (LEN: ❬s❭ = ❬als❭)
-(H: forall (f : nat) (lv : ⦃var⦄) (Z : params),
-       get LV f (⎣ lv ⎦, Z) ->
-       exists b b' : I.block, get L f b /\ get L' (countSome (fst ⊝ take f LV)) b')
-(Get : get (pair ⊜ (getAnn ⊝ als) (fst ⊝ s) ++ LV) f (⎣ lv ⎦, Z))
-  :  exists b b' : I.block, get (mapi I.mkBlock s ++ L) f b /\
-                       get (mapi I.mkBlock (compileF compile (pair ⊜ (getAnn ⊝ als) (fst ⊝ s) ++ LV) s als) ++ L') (countSome (fst ⊝ take f (pair ⊜ (getAnn ⊝ als) (fst ⊝ s) ++ LV))) b'.
+(H: forall (f : nat) (lv : ⦃var⦄),
+       get LV f lv ->
+       exists b b' : I.block, get L f b /\ get L' f b')
+(Get : get (getAnn ⊝ als ++ LV) f lv)
+    :  exists b b' : I.block,
+      get (mapi I.mkBlock s ++ L) f b /\
+      get (mapi I.mkBlock (zip (fun Zs a =>
+                                  (List.filter (fun x => B[x ∈ getAnn a]) (fst Zs),
+                                   compile (pair ⊜ (getAnn ⊝ als ++ LV) (fst ⊝ s ++ ZL)) (snd Zs) a)) s als) ++ L')
+          f b'.
 Proof.
   get_cases Get; inv_get.
-  - exploit compileF_get; eauto.
-    do 2 eexists; split; eauto using get_app, mapi_get_1.
-    eapply get_app. eapply mapi_get_1.
-    erewrite <- getAnn_take_eq; eauto.
+  - edestruct (get_length_eq _ H0 (eq_sym LEN)).
+    do 2 eexists; split; eauto using get_app, mapi_get_1, zip_get.
   - edestruct H as [b [b' [? ?]]]; eauto.
     exists b, b'; split.
-    eapply get_app_right; eauto.
-    rewrite mapi_length. rewrite zip_length2; eauto with len.
-    rewrite map_length.
-    rewrite zip_length2 in H1; eauto with len.
-    rewrite map_length in H1. omega.
-    eapply get_app_right; eauto.
-    rewrite take_app_ge; eauto. rewrite map_app.
-    rewrite countSome_app.
-    rewrite mapi_length.
-    rewrite compileF_length; eauto.
-    rewrite <- getAnn_eq; eauto.
+    + eapply get_app_right; eauto.
+      rewrite mapi_length.
+      rewrite map_length in *. omega.
+    + eapply get_app_right; eauto.
+      rewrite mapi_length.
+      rewrite zip_length2; eauto with len.
+      rewrite map_length in *. omega.
 Qed.
 
-
-Lemma sim_I r L L' V V' s LV lv
-: agree_on eq (oget (getAnn lv)) V V'
--> true_live_sound Imperative LV s lv
--> renILabenv r SR LV L L'
--> (forall (f:nat) lv Z,
-      get LV f (Some lv, Z)
+Lemma sim_I r L L' V V' s ZL LV lv
+: agree_on eq (getAnn lv) V V'
+-> true_live_sound Imperative ZL LV s lv
+-> renILabenv r SR (zip pair LV ZL) L L'
+-> (forall (f:nat) lv,
+      get LV f lv
       -> exists (b b' : I.block),
         get L f b /\
-        get L' (countSome (fst ⊝ (take f LV))) b')
--> sim'r r (L,V, s) (L',V', compile LV s lv).
+        get L' f b')
+-> sim'r r (L,V, s) (L',V', compile (zip pair LV ZL) s lv).
 Proof.
   unfold sim'r. revert_except s.
   sind s; destruct s; simpl; intros; invt true_live_sound; simpl in * |- *.
   - case_eq (exp_eval V e); intros.
     + cases.
-      *  pone_step. instantiate (1:=v).
-         erewrite exp_eval_live; eauto. eapply agree_on_sym; eauto.
-         left. eapply (IH s); eauto. eapply agree_on_update_same. reflexivity.
-         eapply agree_on_incl; eauto.
-      *  eapply sim'_expansion_closed;
-           [ | eapply star2_silent;
-               [ econstructor; eauto | eapply star2_refl ]
-             | eapply star2_refl].
-         eapply (IH s); eauto. eapply agree_on_update_dead; eauto.
-         eapply agree_on_incl; eauto. rewrite <- H10. cset_tac; intuition.
+      * pone_step. instantiate (1:=v).
+        erewrite exp_eval_live; eauto. eapply agree_on_sym; eauto.
+        left. eapply (IH s); eauto. eapply agree_on_update_same. reflexivity.
+        eapply agree_on_incl; eauto.
+      * eapply sim'_expansion_closed;
+          [ | eapply star2_silent;
+              [ econstructor; eauto | eapply star2_refl ]
+            | eapply star2_refl].
+        eapply (IH s); eauto. eapply agree_on_update_dead; eauto.
+        eapply agree_on_incl; eauto.
+        rewrite <- H11. cset_tac; intuition.
     + pfold. econstructor 3; [| eapply star2_refl|]; eauto. stuck.
   - repeat cases.
     + edestruct (exp2bool_val2bool V); eauto; dcr.
       eapply sim'_expansion_closed.
       eapply (IH s1); eauto. eapply agree_on_incl; eauto.
-      eapply H11; congruence.
+      eapply H12; congruence. eapply H6; congruence.
       eapply star2_silent.
       econstructor; eauto. eapply star2_refl.
       eapply star2_refl.
@@ -485,7 +335,7 @@ Proof.
       eapply star2_refl.
     + remember (exp_eval V e). symmetry in Heqo.
       exploit exp_eval_live_agree; eauto.
-      eapply H9. case_eq (exp2bool e); intros; try destruct b; congruence.
+      eapply H10. case_eq (exp2bool e); intros; try destruct b; congruence.
       destruct o. case_eq (val2bool v); intros.
       pfold; econstructor; try eapply plus2O.
       econstructor; eauto. reflexivity.
@@ -499,22 +349,22 @@ Proof.
       stuck.
   - edestruct H2 as [? [? [GetL GetL']]]; eauto.
     remember (omap (exp_eval V) Y). symmetry in Heqo.
-    rewrite (get_nth (None, nil) H5); eauto; simpl.
+    erewrite (get_nth); eauto using zip_get; simpl.
     destruct o.
     + destruct x as [Z1 s1 n1], x0 as [Z2 s2 n2].
       hnf in H1; dcr.
       exploit (@omap_filter_by _ _ _ _ (fun y : var => if [y \In blv] then true else false) _ _ Z Heqo); eauto.
       exploit omap_exp_eval_live_agree; eauto.
       intros. eapply argsLive_liveSound; eauto.
-      edestruct H4 as [[? ?] SIM]; eauto. hnf; eauto.
-      hnf in H12; dcr; subst.
+      edestruct H4 as [[? ?] SIM]; eauto using zip_get. hnf; eauto.
+      hnf in H13; dcr; subst.
       eapply (@sim_Y_left I.state _ I.state _).
       eapply (@sim_Y_right I.state _ I.state _).
       eapply SIM; [ | eapply Heqo | eapply H9 ].
       hnf; simpl. split; eauto.
       exploit (omap_length _ _ _ _ _ Heqo); eauto. split. congruence.
       eauto using agree_on_incl.
-      Focus 4. econstructor; eauto.
+      Focus 4. econstructor; eauto. simpl.
       Focus 2. econstructor; eauto. simpl.
       eapply filter_filter_by_length; eauto.
       * simpl.
@@ -531,53 +381,29 @@ Proof.
     destruct o.
     + pextern_step; eauto using agree_on_update_same, agree_on_incl; try congruence.
     + pno_step.
-  - pone_step. left. eapply IH; eauto.
+  - pone_step. left. rewrite <- zip_app; eauto with len. eapply IH; eauto.
     + simpl in *; eapply agree_on_incl; eauto.
-    + eapply renILabenv_extension; eauto. eauto with len.
+    + rewrite zip_app; eauto with len.
+      eapply renILabenv_extension; eauto. eauto with len.
       * intros. hnf; intros.
-        hnf in H4. dcr.
-        rewrite get_app_lt in H16; eauto using get_range.
-        inv_get.
-        exploit (compileF_get ((pair ⊜ (getAnn ⊝ als) (fst ⊝ s) ++ LV) )); eauto.
-        erewrite <- getAnn_take_eq in H10; eauto.
-        get_functional. clear EQ0.
-        hnf in H14; dcr; subst.
+        hnf in H4. subst n'. inv_get. simpl.
+        hnf in H13; dcr; subst. simpl.
+        rewrite <- zip_app; eauto with len.
         eapply IH; eauto.
-        rewrite EQ. simpl.
         eapply agree_on_update_filter'; eauto.
         exploit H7; eauto using zip_get.
-        rewrite <- EQ. eapply zip_get; eauto using map_get.
-        exploit H9; eauto.
-        intros.
-        eapply inv_extend; eauto.
+        rewrite zip_app; eauto with len.
+        intros. eapply inv_extend; eauto.
       * hnf; intros.
-        hnf in H3. dcr.
-        rewrite get_app_lt in H14; eauto with len.
-        inv_get. simpl; unfold ParamRel; simpl.
-        exploit (compileF_get ((pair ⊜ (getAnn ⊝ als) (fst ⊝ s) ++ LV) )); eauto.
-        erewrite <- getAnn_take_eq in H6; eauto.
-        get_functional. eauto.
-      * intros. rewrite compileF_length; eauto.
+        hnf in H3. dcr. inv_get.
+        simpl; unfold ParamRel; simpl; eauto.
+      * intros.
         hnf in H3; dcr; subst.
-        rewrite get_app_lt in H10;
-          [| rewrite zip_length2; eauto with len; rewrite map_length; omega].
-        inv_get.
-        erewrite <- getAnn_take_eq; eauto.
-        rewrite map_take.
-        erewrite (take_eta n (getAnn ⊝ als)) at 2.
-        rewrite countSome_app.
-        erewrite <- get_eq_drop; eauto using map_get_1.
-        rewrite EQ1. simpl; omega.
-      * intros. rewrite compileF_length; eauto.
+        eauto with len.
+      * intros.
         hnf in H3; dcr; subst.
-        rewrite map_take. rewrite map_app.
-        rewrite map_zip.
-        rewrite zip_map_fst; eauto with len.
-        rewrite take_app_ge. rewrite countSome_app. omega.
-        rewrite map_length. omega.
-      * simpl. rewrite compileF_length; eauto.
-        rewrite map_zip.
-        rewrite zip_map_fst; eauto with len.
+        rewrite zip_length2; eauto.
+      * simpl. eauto with len.
     + intros; eapply inv_extend; eauto.
 Qed.
 
